Added New View message.
We have added the action for the Primary of a View to
select a set of 2F+1 View Change messages and to pack
them inside a NewViewMsg. The Primary can then send
this message to the peers so that Replicas will be able
to go to the next phase of the View Change process.

messages.dfy
@@ -30,12 +30,25 @@ module Messages {
     }
   }
 
+  datatype ViewChangeMsgsSelectedByPrimary = ViewChangeMsgsSelectedByPrimary(msgs:set<Network.Message<Message>>) {
+    predicate valid(view:ViewNum, quorumSize:nat) {
+      && |msgs| > 0
+      && (forall v | v in msgs :: && v.payload.ViewChangeMsg? 
+                                  && v.payload.newView == view) // All the ViewChange messages have to be for the same View. 
+      && (forall v1, v2 | && v1 in msgs
+                          && v2 in msgs
+                          && v1 != v2
+                            :: v1.sender != v2.sender) // unique senders
+      && |msgs| >= quorumSize
+    }
+  }
+
   // Define your Message datatype here.
   datatype Message = | PrePrepare(view:ViewNum, seqID:SequenceID, clientOp:ClientOperation)
                      | Prepare(view:ViewNum, seqID:SequenceID, clientOp:ClientOperation)
                      | Commit(view:ViewNum, seqID:SequenceID, clientOp:ClientOperation)
                      | ClientRequest(clientOp:ClientOperation)
                      | ViewChangeMsg(newView:ViewNum, certificates:imap<SequenceID, PreparedCertificate>) // omitting last stable because we don't have checkpointing yet.
-
+                     | NewViewMsg(newView:ViewNum, vcMsgs:ViewChangeMsgsSelectedByPrimary)
   // ToDo: ClientReply
 }
